coq/Common/AMap.v
@@ -1,0 +1,102 @@
+Require Import Coq.ZArith.BinInt.
+Require Import Coq.FSets.FMapAVL.
+
+From ExtLib.Data Require Import List.
+From ExtLib.Structures Require Import Monad Monads Traversable.
+
+From Coq.Lists Require Import List. (* after exltlib *)
+
+From CheriCaps.Morello Require Import Capabilities.
+
+From Common Require Import Utils.
+
+Local Open Scope type_scope.
+Local Open Scope list_scope.
+Local Open Scope monad_scope.
+
+Import MonadNotation.
+
+Require Import Coq.FSets.FMapFacts.
+
+Module AMap := FMapAVL.Make(AddressValue_as_OT).
+Module Import AP := FMapFacts.WProperties_fun(AddressValue_as_OT)(AMap).
+
+Fixpoint amap_range_init {T} (a0:AddressValue.t) (n:nat) (step:Z) (v:T) (m:AMap.t T) : AMap.t T
+  :=
+  match n with
+  | O => m
+  | S n =>
+      let m := amap_range_init a0 n step v m in
+      AMap.add (AddressValue.with_offset a0 (Z.mul (Z.of_nat n) step)) v m
+  end.
+
+Definition amap_update_element
+  {A:Type}
+  (key: AddressValue.t)
+  (v: A)
+  (m: AMap.t A)
+  : (AMap.t A)
+  :=
+  AMap.add key v (AMap.remove key m).
+
+(** [update key f m] returns a map containing the same bindings as
+  [m], except for the binding of [key]. Depending on the value of [y]
+  where [y] is [f (find_opt key m)], the binding of [key] is added,
+  removed or updated. If [y] is [None], the binding is removed if it
+  exists; otherwise, if [y] is [Some z] then key is associated to [z]
+  in the resulting map. *)
+Definition amap_update
+  {A:Type}
+  (key: AddressValue.t)
+  (f: option A -> option A)
+  (m: AMap.t A)
+  : (AMap.t A)
+  :=
+  let y := f (AMap.find key m) in
+  let m' := AMap.remove key m in (* could be optimized, as removal may be unecessary in some cases *)
+  match y with
+  | None => m'
+  | Some z => AMap.add key z m'
+  end.
+
+Definition amap_sequence
+  {A: Type}
+  {m: Type -> Type}
+  {M: Monad m}
+  (mv: AMap.t (m A)): m (AMap.t A)
+  :=
+  let (kl,vl) := List.split (AMap.elements mv) in
+  vl' <- sequence (F:=m) (T:=list) vl ;;
+  ret (of_list (combine kl vl')).
+
+(** Adds elements of given [list] to a [map] starting at [addr]. *)
+Definition amap_add_list_at
+  {T:Type}
+  (map: AMap.t T)
+  (list: list T)
+  (addr: AddressValue.t)
+  : AMap.t T
+  :=
+  let ilist := mapi (fun (i: nat) (v: T) => ((AddressValue.with_offset addr (Z.of_nat i)), v)) list in
+  List.fold_left (fun acc '(k, v) =>  AMap.add k v acc) ilist map.
+
+(* Monadic mapi *)
+Definition amap_mmapi
+  {A B : Type}
+  {m : Type -> Type}
+  {M : Monad m}
+  (f : AMap.key -> A -> m B) (zm: AMap.t A)
+  : m (AMap.t B)
+  :=
+  amap_sequence (AMap.mapi f zm).
+
+Definition amap_find_first {A:Type} (f:AMap.key -> A -> bool) (m:AMap.t A): option (AMap.key * A)
+  :=
+  AMap.fold (fun k v (acc:option (AMap.key * A)) =>
+               match acc with
+               | None => if f k v
+                        then Some (k, v)
+                        else None
+               | Some _ => acc
+               end)
+    m None.
